src/RoseTree.v
@@ -39,13 +39,6 @@ End list_size.
 
 Require Import List.
 (* end hide *)
-(** To demonstrate nested well-founded recursive definitions, we take a
-  well-known example from the literature: rose trees.  We will define a
-  recursive function gathering the elements in a [rose] tree in an efficient
-  way, using nested well-founded recursion instead of the guardedness check of %\Coq%.
-  The [rose] trees are defined as trees whose nodes contain lists of trees,
-  i.e. forests. *)
-
 (** To solve measure subgoals *)
 #[local] Hint Extern 4 (_ < _) => simpl; lia : rec_decision.
 Obligation Tactic := CoreTactics.equations_simpl; try (simpl; lia); try typeclasses eauto with rec_decision.
@@ -88,23 +81,6 @@ Section RoseTree.
         + eapply IHNODES. apply Hin.
     Qed.
   End Induction.
-
-  (** As explained at the beginning of this section, however, if we want
-      to program more complex recursions, or rearrange our terms
-      slightly and freely perform dependent pattern-matching, the
-      limited syntactic guardness check will quickly get in our way.
-
-      Using a _nested_ [where] clause and the support of %\Equations% for
-      well-founded recursion, we can define the following function
-      gathering the elements in a rose tree efficiently: *)
-
-  Equations elements (r : rose) (acc : list rose) : list rose by wf (size r) lt :=
-  elements (node _ l) acc := aux l _
-    where aux x (H : list_size size x < size (node _ l)) : list rose by wf (list_size size x) lt :=
-    aux nil _ := acc;
-    aux (cons x xs) H := elements x (aux xs _).
-
-  Definition elems r := elements r nil.
 
   Equations rose_eqb (r1 r2 : rose) : bool by wf (size r1) lt :=
     rose_eqb (node n1 []) (node n2 []) := Nat.eqb n1 n2;
@@ -157,6 +133,11 @@ Section RoseTree.
     - constructor 2. intro. subst. rewrite rose_eqb_refl in Heqb0. inversion Heqb0.
   Qed.
 
+  Lemma rose_eq_dec : forall (a b : rose), {a = b} + {a <> b}.
+  Proof.
+    intros. apply (reflect_dec _ _ (rose_eqb_spec _ _)).
+  Qed.
+
   Lemma rose_eqb_trans : forall a b c,
       rose_eqb a b = true ->
       rose_eqb b c = true ->
@@ -166,14 +147,15 @@ Section RoseTree.
   Qed.
 
   Equations parent (r1 : rose) (r2 : rose) : bool by wf (size r2) lt :=
-    parent a (node _ l) := match find (rose_eqb a) l with
-                           | Some _ => true
-                           | None => aux a l _
-                         end
-  where aux r1 (l' : list rose) (H : list_size size l' < size (node _ l)) : bool
+    parent r1 (node n l) := match find (rose_eqb r1) l with
+                           | Some _ => true (* found directly at this level *)
+                           | None => aux r1 l _ (* find at a lower level *)
+                           end
+  (* find in the lists in each [rose] in [l'] *)
+  where aux r1' (l' : list rose) (H : list_size size l' < size (node _ l)) : bool
     by wf (list_size size l') lt :=
     aux _ nil _ := false;
-    aux a' (cons x xs) H := parent a' x || aux a' xs _.
+    aux r1' (x :: xs) H := parent r1' x || aux r1' xs _.
 
   Goal parent (node 1 nil) (node 1 [node 1 [node 2 nil; node 1 nil]]) = true. auto. Qed.
   Goal parent (node 1 nil) (node 1 [node 1 [node 2 nil; node 3 nil]]) = false. auto. Qed.
@@ -182,8 +164,94 @@ Section RoseTree.
   Goal parent (node 1 [node 2 nil])
        (node 1 [node 1 [node 2 nil; node 3 nil]]) = false. auto. Qed.
 
-  (**
-    The function is nesting a well-founded recursion inside
+  Lemma parent_foo r n x xs :
+    parent r (node n xs) = true ->
+    parent r (node n (x :: xs)) = true.
+  Proof.
+    simp parent. simpl.
+    intros. destruct (rose_eqb r x); auto. destruct (find (rose_eqb r) xs); auto.
+  Abort.
+
+  (* todo: rewrite this with parent in last case, then try using parents_elim *)
+  Lemma parent_cases r n x xs :
+    parent r (node n (x :: xs)) = true ->
+    (exists i, find (rose_eqb r) (x :: xs) = Some i) \/ parent r x = true \/
+      parent_unfold_clause_1_aux r n (x :: xs) r xs
+        (parent_obligations_obligation_3 n (x :: xs) x xs
+           (parent_obligations_obligation_5 n (x :: xs))) = true.
+  Proof.
+    intros. simp parent in H.
+    destruct (find (rose_eqb r) (x :: xs)) eqn:Hfind; auto.
+    left. eexists. auto.
+    right.
+    apply orb_prop in H. destruct H.
+    left; auto. right. auto.
+  Qed.
+
+  Lemma parent_trans (r1 r2 r3 : rose) :
+    parent r1 r2 = true ->
+    parent r2 r3 = true ->
+    parent r1 r3 = true.
+  Proof.
+    revert r2.
+    (* revert r1 r2 r3. *)
+    eapply (parent_elim
+              (fun r1 r2 b => forall r',
+                   parent r1 r' = true ->
+                   parent r' r2 = true ->
+                   (* parent r1 r2 = b -> *)
+                   b = true)
+              (fun r1 n l r' l' H b => forall r'',
+                   r1 = r' ->
+                   parent r1 r'' = true ->
+                   parent r'' (node n l') = true ->
+                   match find (rose_eqb r1) l' with
+                   | Some _ => true
+                   | None => b
+                   end = true
+           )).
+    - intros. eapply H; eauto.
+    - intros. inversion H2.
+    - clear r1 r3. intros. subst. unfold find. fold (find (rose_eqb r1') xs).
+      destruct (rose_eqb r1' x) eqn:Heqb; auto.
+      destruct (find (rose_eqb r1') xs) eqn:Hfind; auto.
+      apply parent_cases in H4. destruct H4 as [? | [? | ?]].
+      + destruct H2. unfold find in H2. fold (find (rose_eqb r'') xs) in H2.
+        destruct (rose_eqb r'' x) eqn:?.
+        * inversion H2. subst.
+          rewrite <- (reflect_iff _ _ (rose_eqb_spec r'' x0)) in Heqb0. subst.
+          rewrite H3. auto.
+        * erewrite H1; eauto.
+          rewrite orb_true_r. auto.
+          simp parent. rewrite H2. auto.
+      + erewrite H0; eauto.
+      + erewrite H1; eauto. rewrite orb_true_r. auto.
+        (* eapply parent_foo. *)
+          (* simp parent in H4. rewrite H *)
+      (* erewrite H1. admit. *)
+      (* apply H2. *)
+
+      (* simp parent in H3. unfold find in H3. fold (find (rose_eqb r'') xs) in H3. rewrite Hfind in H3. *)
+  Admitted.
+
+    (** As explained at the beginning of this section, however, if we want
+      to program more complex recursions, or rearrange our terms
+      slightly and freely perform dependent pattern-matching, the
+      limited syntactic guardness check will quickly get in our way.
+
+      Using a _nested_ [where] clause and the support of %\Equations% for
+      well-founded recursion, we can define the following function
+      gathering the elements in a rose tree efficiently: *)
+
+  Equations elements (r : rose) (acc : list rose) : list rose by wf (size r) lt :=
+  elements (node n l) acc := aux l _
+    where aux x (H : list_size size x < size (node _ l)) : list rose by wf (list_size size x) lt :=
+    aux nil _ := acc;
+    aux (cons x xs) H := elements x (aux xs _).
+
+  Definition elems r := elements r nil.
+
+  (** The function is nesting a well-founded recursion inside
     another one, based on the measure of [rose] trees and lists ([MR R
     f] is a combinator for [λ x y, R (f x) (f y)]).  The termination
     of this definition is ensured solely by logical means, it does not
